rt haskell+refine+crefine: prove finaliseCap_ccorres
Signed-off-by: Michael McInerney <michael.mcinerney@proofcraft.systems>

spec/haskell/src/SEL4/Kernel/Thread.lhs
@@ -141,6 +141,7 @@ When a thread is suspended, either explicitly by a TCB invocation or implicitly 
 > suspend :: PPtr TCB -> Kernel ()
 > suspend target = do
 >     stateAssert sym_refs_asrt "`sym_refs (state_refs_of' s)`"
+>     stateAssert weak_sch_act_wf_asrt "assert that `weak_sch_act_wf` holds"
 >     cancelIPC target
 >     state <- getThreadState target
 >     if state == Running then updateRestartPC target else return ()
